ended up writing a seqSliceSlice lemma

lib/Marshalling/TupleMarshalling.i.dfy
@@ -3,7 +3,202 @@ include "MarshalledAccessors.i.dfy"
 abstract module Tuple2Marshalling refines Marshalling {
   import FstMarshalling : Marshalling
   import SndMarshalling : Marshalling
+  import SizeMarshalling : IntegerMarshalling
 
   type UnmarshalledType = (FstMarshalling.UnmarshalledType, SndMarshalling.UnmarshalledType)
+  type SizeType = SizeMarshalling.UnmarshalledType
 
+  function method fstSizeSize(): uint64
+  {
+    SizeMarshalling.Int.Size() as uint64
+  }
+
+  predicate parsable(data: mseq<byte>)
+  {
+    var fstSizeSize := fstSizeSize() as int;
+    && |data| >= fstSizeSize
+    && SizeMarshalling.parsable(data[..fstSizeSize])
+    && var size := SizeMarshalling.Int.toInt(SizeMarshalling.parse(data[..fstSizeSize]));
+    && size >= 0
+    && |data| >= fstSizeSize + size
+    && FstMarshalling.parsable(data[fstSizeSize..fstSizeSize + size])
+    && SndMarshalling.parsable(data[fstSizeSize + size..])
+  }
+
+  function parse(data: mseq<byte>) : UnmarshalledType
+    // requires parsable(data)
+  {
+    var fstSizeSize := fstSizeSize() as int;
+    var size := SizeMarshalling.Int.toInt(SizeMarshalling.parse(data[..fstSizeSize]));
+    var fstElm := FstMarshalling.parse(data[fstSizeSize..fstSizeSize + size]);
+    var sndElm := SndMarshalling.parse(data[fstSizeSize + size..]);
+    (fstElm, sndElm)
+  }
+
+  method TryParse(data: mseq<byte>) returns (ovalue: Option<UnmarshalledType>)
+    // ensures parsable(data) <==> ovalue.Some?
+    // ensures parsable(data) ==> ovalue.value == parse(data)
+  {
+    var fstSizeSize := fstSizeSize();
+
+    if fstSizeSize > |data| as uint64 {
+      return None;
+    }
+
+    var sizeOvalue := SizeMarshalling.TryParse(data[..fstSizeSize]);
+    
+    if sizeOvalue.None? {
+      return None;
+    }
+
+    if !SizeMarshalling.Int.fitsInUint64(sizeOvalue.value) {
+      return None;
+    }
+
+    var size := SizeMarshalling.Int.toUint64(sizeOvalue.value);
+
+    if size > |data| as uint64 - fstSizeSize {
+      return None;
+    }
+
+    var fstOvalue := FstMarshalling.TryParse(data[fstSizeSize..fstSizeSize + size]);
+    var sndOvalue := SndMarshalling.TryParse(data[fstSizeSize + size..]);
+    if fstOvalue.Some? && sndOvalue.Some? {
+      ovalue := Some((fstOvalue.value, sndOvalue.value));
+    } else {
+      ovalue := None;
+    }
+  }
+
+  method Parsable(data: mseq<byte>) returns (p: bool)
+    // ensures p == parsable(data)
+  {
+    var fstSizeSize := fstSizeSize();
+
+    if fstSizeSize > |data| as uint64 {
+      return false;
+    }
+
+    var sizeOvalue := SizeMarshalling.TryParse(data[..fstSizeSize]);
+    
+    if sizeOvalue.None? {
+      return false;
+    }
+
+    if !SizeMarshalling.Int.fitsInUint64(sizeOvalue.value) {
+      return false;
+    }
+
+    var size := SizeMarshalling.Int.toUint64(sizeOvalue.value);
+
+    if size > |data| as uint64 - fstSizeSize {
+      return false;
+    }
+
+    var fstParsable := FstMarshalling.Parsable(data[fstSizeSize..fstSizeSize + size]);
+    var sndParsable := SndMarshalling.Parsable(data[fstSizeSize + size..]);
+
+    return fstParsable && sndParsable;
+  }
+
+  method Parse(data: mseq<byte>) returns (value: UnmarshalledType)
+    // requires parsable(data)
+    // ensures value == parse(data)
+  {
+    var fstSizeSize := fstSizeSize();
+
+    var isize := SizeMarshalling.Parse(data[..fstSizeSize]);
+    var size := SizeMarshalling.Int.toUint64(isize);
+
+    var fstValue := FstMarshalling.Parse(data[fstSizeSize..fstSizeSize + size]);
+    var sndValue := SndMarshalling.Parse(data[fstSizeSize + size..]);
+    value := (fstValue, sndValue);
+  }
+
+  predicate marshallable(value: UnmarshalledType)
+  {
+    && var (fstValue, sndValue) := value;
+    && FstMarshalling.marshallable(fstValue)
+    && SndMarshalling.marshallable(sndValue)
+    && var size := FstMarshalling.size(fstValue);
+    && SizeMarshalling.Int.MinValue() <= size < SizeMarshalling.Int.UpperBound()
+    && SizeMarshalling.marshallable(SizeMarshalling.Int.fromInt(size))
+  }
+
+  function size(value: UnmarshalledType) : nat
+  {
+    var (fstValue, sndValue) := value;
+    fstSizeSize() as nat + FstMarshalling.size(fstValue) + SndMarshalling.size(sndValue)
+  }
+
+  method Size(value: UnmarshalledType) returns (sz: uint64)
+    // requires marshallable(value)
+    // requires size(value) < Uint64UpperBound()
+    // ensures sz as nat == size(value)
+  {
+    var (fstValue, sndValue) := value;
+    var fstSz := FstMarshalling.Size(fstValue);
+    var sndSz := SndMarshalling.Size(sndValue);
+    sz := fstSizeSize() + fstSz + sndSz;
+  }
+
+  lemma seqSliceSlice(s: mseq<byte>, a: uint64, b: uint64, c: uint64, d: uint64)
+    requires a <= b <= |s| as uint64;
+    requires c <= d <= b - a;
+    requires a + d <= b;
+    ensures s[a..b][c..d] == s[a + c..a + d];
+  {
+    assert s[a..b] == s[a..b];
+    assert s[a..b][c..] == s[a + c..b];
+    assert s[a..b][c..d] == s[a + c..a + d];
+  }
+
+  method Marshall(value: UnmarshalledType, linear data: mseq<byte>, start: uint64)
+    returns (linear newdata: mseq<byte>, end: uint64)
+  {
+    ghost var fstSzSz : uint64 := fstSizeSize();
+    var (fstValue, sndValue) := value;
+    var fstSz := FstMarshalling.Size(fstValue);
+    newdata, end := SizeMarshalling.Marshall(SizeMarshalling.Int.fromUint64(fstSz), data, start);
+    ghost var newdata1 :seq<byte> := newdata;
+    ghost var end1 := end;
+
+    newdata, end := FstMarshalling.Marshall(fstValue, newdata, end);
+    ghost var newdata2 :seq<byte> := newdata;
+    ghost var end2 := end;
+
+    newdata, end := SndMarshalling.Marshall(sndValue, newdata, end);
+
+    assert start + fstSzSz == end1;
+    assert end1 + fstSz == end2;
+
+    assert newdata1[start..end1] == newdata[start..end1];
+    assert newdata2[end1..end2] == newdata[end1..end2];
+
+    // calc == {
+    //   newdata[start..end][fstSzSz..end2 - start];
+    //   {
+    //     assert end1 + fstSz == end2;
+    //   }
+    //   newdata[start..end][fstSzSz.. end1 + fstSz - start];
+    //   {
+    //     assert start + fstSzSz == end1;
+    //   }
+    //   newdata[start..end][fstSzSz..fstSzSz + fstSz];
+    //   {
+    //     // assume start + fstSzSz + fstSz < end;
+    //   }
+    //   newdata[start + fstSzSz..start + fstSzSz + fstSz];
+    // }
+
+    seqSliceSlice(newdata, start, end, fstSzSz, end2 - start);
+    assert newdata[start..end][fstSzSz..end2 - start] == newdata[end1.. end2];
+    // assume newdata[start..end][fstSzSz..end2 - start] == newdata[end1 .. end2];
+
+    ghost var size := SizeMarshalling.Int.toInt(SizeMarshalling.parse(newdata[start..end1]));
+    SizeMarshalling.Int.fromtoInverses();
+
+    assert newdata[start..end][..fstSzSz] == newdata[start..end1];
+    assert size == fstSz as int;
+  }
 }
